progs/VSUpile/simple_verif_apile.v
@@ -22,12 +22,12 @@ cancel.
 Qed.
 
   Lemma MyInitData gv (H: headptr (gv _a_pile)):
-        initialize.gv_globvar2pred gv (_a_pile, v_a_pile)
+        globvar2pred gv (_a_pile, v_a_pile)
         |-- apile nil gv.
   Proof.
   eapply derives_trans; [ | apply make_apile; auto].
-  unfold initialize.gv_globvar2pred, apile. simpl.
-  rewrite predicates_sl.sepcon_emp. forget (gv _a_pile) as p.
+  unfold globvar2pred, apile. simpl.
+  rewrite sepcon_emp. forget (gv _a_pile) as p.
   erewrite <- (mapsto_data_at'' Ews); auto.
   apply derives_refl.
   Qed.
