progs/VSUpile/simple_verif_onepile.v
@@ -59,11 +59,11 @@ intros. cancel.
 Qed.
 
   Lemma onepile_Init_aux gv: headptr (gv _the_pile) ->
-    initialize.gv_globvar2pred gv (_the_pile, v_the_pile)
+    globvar2pred gv (_the_pile, v_the_pile)
     |-- data_at_ Ews (tptr (Tstruct _pile noattr)) (gv _the_pile).
   Proof. intros.
-    unfold initialize.gv_globvar2pred. simpl.
-         rewrite predicates_sl.sepcon_emp.
+    unfold globvar2pred. simpl.
+         rewrite sepcon_emp.
     destruct H as [b Hb]; rewrite Hb in *.
     eapply derives_trans. 
     + apply mapsto_zeros_memory_block. apply writable_readable. apply writable_Ews.
@@ -73,7 +73,7 @@ Qed.
   Qed.
 
   Lemma onepile_Init_aux2 gv: headptr (gv _the_pile) ->
-    initialize.gv_globvar2pred gv (_the_pile, v_the_pile)
+    globvar2pred gv (_the_pile, v_the_pile)
     |--  onepile None gv.
   Proof. intros. sep_apply onepile_Init_aux. apply make_onepile; trivial. Qed.
 
