progs/VSUpile/verif_linked_main.v
@@ -182,7 +182,7 @@ Qed.
 Lemma main_sub: funspec_sub (snd (main_inst_spec M (MyInitPred (ONEPILE M) (APILE M))))
                              (snd mainspec).
 Proof. do_funspec_sub. unfold main_pre; simpl; Intros; subst. clear. 
-  Exists w emp. unfold gglobvars2pred; simpl.
+  Exists (initialize.genviron2globals g) emp. unfold globvars2pred; simpl.
   unfold globvars2pred, lift2; Intros. simpl. entailer!.
   + intros. entailer!.
   + rewrite sepcon_comm; apply sepcon_derives.
@@ -192,15 +192,16 @@ Proof. do_funspec_sub. unfold main_pre; simpl; Intros; subst. clear.
       * eapply derives_trans. apply mapsto_zeros_memory_block.
         apply writable_readable. apply writable_Ews.
         rewrite memory_block_isptr; Intros.
-        apply global_is_headptr in H. entailer!.
-      * unfold initialize.gv_globvar2pred. simpl.
-        rewrite predicates_sl.sepcon_emp. apply derives_refl.
-      (*unfold globvar2pred; simpl. sep_apply mapsto_zeros_isptr; Intros.
-      * apply writable_readable. apply writable_Ews.
-      * apply global_is_headptr in H.
-        Check verif_onepile.make_onepile. , sepcon_emp by trivial.
-      erewrite <- (mapsto_data_at''); trivial. apply derives_refl.*)
-    - unfold globvar2pred; simpl. rewrite mapsto_isptr; Intros. apply global_is_headptr in H.
+        apply prop_right.
+        unfold initialize.genviron2globals in *.
+        destruct (Map.get g onepile._the_pile); try contradiction; auto.
+        eexists; reflexivity.
+      * auto.
+    - unfold globvar2pred; simpl. rewrite mapsto_isptr; Intros.
+       assert (headptr (initialize.genviron2globals g apile._a_pile)).
+        unfold initialize.genviron2globals in *.
+        destruct (Map.get g apile._a_pile); try contradiction; auto.
+        eexists; reflexivity.
       rewrite <- verif_apile.make_apile, sepcon_emp by trivial.
       erewrite <- (mapsto_data_at''); trivial. apply derives_refl.
 Qed.
